Zcash/Circuits/Halo2/Witness.lean
@@ -12,11 +12,4 @@ variable {F : Type} [FiniteField F]
 def extractWitness (assignment : ProofAssignment F) : top.PrivateWitness :=
   top.extractPrivate top.config (top.placedEnvironment assignment)
 
-/-- Source constraints establish the specification for the extracted witness. -/
-theorem spec_of_constraints (assignment : ProofAssignment F)
-    (hconstraints : Constraints top.placement (top.environment assignment) top.operations 0) :
-    top.Spec (top.extractPublicInput (top.environment assignment))
-      (top.extractWitness assignment) :=
-  top.soundness assignment hconstraints
-
 end Halo2.TopLevelCircuit
